

\section{Session 7: Homogenization - Multiscale}

\begin{equation}\label{key}
\nabla\cdot(C(x,y)\nabla^s u)=\rho b
\end{equation}
Kinetics assumptions
\begin{equation}\label{eq:kinetic1}
\epsilon_u(x,y)=\epsilon(x)+\tilde{\epsilon_u}(x,y)
\end{equation}
\begin{equation}\label{eq:kinetic2}
\frac{1}{\Omega_u}\int_{\Omega_u}^{}\tilde{\epsilon_u}(x,y)=0
\end{equation}
By inserting Equation \ref{eq:kinetic1} into Equation \ref{eq:kinetic2}:
\begin{equation}\label{key}
\frac{1}{\Omega_u}\int_{\Omega_u}^{}\left(\epsilon_u(x,y)-\epsilon(x)\right)=0 \rightarrow \frac{1}{\Omega_u}\int_{\Omega_u}^{}\epsilon_u(x,y)=\frac{1}{\Omega_u}\epsilon(x)\int_{\Omega_u}^{}\delta\Omega_u 
\end{equation}
Hill-Mandel Principle
\begin{equation}\label{key}
\sigma\cdot\delta_{\epsilon}=\frac{1}{|\Omega_u|}\int\sigma_u\colon\delta_{\epsilon} \forall\delta_{\epsilon}\delta_{\epsilon_m}
\end{equation}


\clearpage























